Refactoring of the refinement proposition
There is now a separate `REL e1 << e2 @ E : A` proposition,
on top of which we define the semantic typing judgement.

All the tactics work on the `REL .. << ..` proposition, and we use it
to prove the fundamental property. This means that we have to deal
with substitutions whenever we are doing something with the typing
judgement, but in practice this is not so bad.

Also added and updated: the counters refinement example.

theories/logic/model.v
@@ -6,8 +6,9 @@
 From iris.heap_lang Require Export lifting metatheory.
 From iris.base_logic.lib Require Import invariants.
 From iris.algebra Require Import list gmap.
-From iris.heap_lang Require Import notation proofmode.
-From reloc Require Import prelude.tactics logic.spec_rules prelude.ctx_subst.
+From iris.heap_lang Require Export lang notation.
+From iris.heap_lang Require Import proofmode.
+From reloc Require Import prelude.properness logic.spec_rules prelude.ctx_subst.
 From reloc Require Export logic.spec_ra.
 
 (** Semantic intepretation of types *)
@@ -134,122 +135,30 @@ End semtypes.
 (* Nice notations *)
 Notation "()" := lty2_unit : lty_scope.
 Infix "→" := lty2_arr : lty_scope.
+Infix "×" := lty2_prod (at level 80) : lty_scope.
 Notation "'ref' A" := (lty2_ref A) : lty_scope.
-
-(* The semantic typing judgment *)
-Definition env_ltyped2 `{relocG Σ} (Γ : gmap string (lty2 Σ))
-    (vs : gmap string (val*val)) : iProp Σ :=
-  (⌜ ∀ x, is_Some (Γ !! x) ↔ is_Some (vs !! x) ⌝ ∧
-  [∗ map] i ↦ Avv ∈ map_zip Γ vs, lty2_car Avv.1 Avv.2.1 Avv.2.2)%I.
-
-(** todo move this to prelude *)
-Section big_opm.
-  Context `{Countable K} {A : ofeT}.
-  Context `{Monoid M o}.
-
-  Infix "`o`" := o (at level 50, left associativity).
-  Implicit Types m : gmap K A.
-  Implicit Types f g : K → A → M.
-
-  Global Instance big_opM_ne2 n `{Proper _ (dist n ==> dist n ==> dist n) o} :
-    Proper (pointwise_relation _ (dist n ==> dist n) ==> dist n ==> dist n)
-           (big_opM o (K:=K) (A:=A)).
-  Proof.
-    intros f g Hf m1.
-    induction m1 as [|i x m Hnone IH] using map_ind.
-    { intros m2 Hm2. rewrite big_opM_empty.
-      induction m2 as [|j y m2 ? IH2] using map_ind.
-      - by rewrite big_opM_empty.
-      - exfalso.
-        specialize (Hm2 j). revert Hm2.
-        rewrite lookup_insert lookup_empty /=. by inversion 1. }
-    intros m2 Hm2.
-    assert (is_Some (m2 !! i)) as [y Hy].
-    { specialize (Hm2 i). revert Hm2. rewrite lookup_insert=>Hm2.
-      destruct (m2 !! i); first naive_solver.
-      inversion Hm2. }
-    replace m2 with (<[i:=y]>(delete i m2)).
-    - rewrite !big_opM_insert // /=; last by apply lookup_delete.
-      f_equiv.
-      + apply Hf. specialize (Hm2 i). revert Hm2.
-        rewrite Hy lookup_insert //. by inversion 1.
-      + apply IH=> j.
-        destruct (decide (j = i)) as [->|?].
-        * by rewrite lookup_delete Hnone.
-        * rewrite lookup_delete_ne//. specialize (Hm2 j).
-          revert Hm2. by rewrite lookup_insert_ne.
-    - rewrite insert_delete insert_id //.
-  Qed.
-
-End big_opm.
-
-(** todo, move to iris *)
-Instance option_mbind_ne {A B : ofeT} n :
-  Proper (((dist n) ==> (dist n)) ==> (dist n) ==> (dist n)) (@option_bind A B).
-Proof. destruct 2; simpl; try constructor; auto. Qed.
-
-(** todo move somewhere *)
-Instance map_zip_with_ne {K} {A B C : ofeT} (f : A → B → C)
-  `{Countable K} `{!EqDecision K} n :
-  Proper (dist n ==> dist n ==> dist n) f →
-  Proper (dist n ==> dist n ==> dist n)
-    (@map_zip_with (gmap K) _ _ _ _ f).
-Proof.
-  intros Hf m1 m2 Hm2 m1' m2' Hm2' i.
-  rewrite !map_lookup_zip_with. f_equiv =>//.
-  intros x1 x2 Hx2. f_equiv =>//.
-  intros y1 y2 Hy2. repeat f_equiv =>//.
-Qed.
-
-Instance env_ltyped2_ne `{relocG Σ} n :
-  Proper (dist n ==> (=) ==> dist n) env_ltyped2.
-Proof.
-  intros Γ Γ' HΓ ? vvs ->.
-  rewrite /env_ltyped2.
-  f_equiv.
-  - f_equiv.
-    split;
-      intros Hvvs x; specialize (HΓ x); rewrite -(Hvvs x);
-      by apply (is_Some_ne n).
-  - apply big_opM_ne2; first apply _.
-    + by intros x A B ->.
-    + apply map_zip_with_ne=>//. apply _.
-Qed.
-
-Instance env_ltyped2_proper `{relocG Σ} :
-  Proper ((≡) ==> (=) ==> (≡)) env_ltyped2.
-Proof. solve_proper_from_ne. Qed.
 
 Section refinement.
   Context `{relocG Σ}.
 
-  Definition refines_def  (E : coPset)
-           (Γ : gmap string (lty2 Σ))
+  Definition refines_def (E : coPset)
            (e e' : expr) (A : lty2 Σ) : iProp Σ :=
-    (∀ vvs ρ, spec_ctx ρ -∗
-              env_ltyped2 Γ vvs -∗
-              interp_expr E (subst_map (fst <$> vvs) e)
-                            (subst_map (snd <$> vvs) e')
-                            A)%I.
+    (∀ ρ, spec_ctx ρ -∗ interp_expr E e e' A)%I.
   Definition refines_aux : seal refines_def. Proof. by eexists. Qed.
   Definition refines := unseal refines_aux.
   Definition refines_eq : refines = refines_def :=
     seal_eq refines_aux.
 
   Global Instance refines_ne E n :
-    Proper ((dist n) ==> (=) ==> (=) ==> (dist n) ==> (dist n)) (refines E).
-  Proof.
-    rewrite refines_eq /refines_def.
-    solve_proper.
-  Qed.
+    Proper ((=) ==> (=) ==> (dist n) ==> (dist n)) (refines E).
+  Proof. rewrite refines_eq /refines_def. solve_proper. Qed.
 
   Global Instance refines_proper E  :
-    Proper ((≡) ==> (=) ==> (=) ==> (≡) ==> (≡)) (refines E).
+    Proper ((=) ==> (=) ==> (≡) ==> (≡)) (refines E).
   Proof. solve_proper_from_ne. Qed.
 End refinement.
 
 Notation "⟦ A ⟧ₑ" := (λ e e', interp_expr ⊤ e e' A).
-Notation "⟦ Γ ⟧*" := (env_ltyped2 Γ).
 
 Section semtypes_properties.
   Context `{relocG Σ}.
@@ -299,76 +208,35 @@ Section semtypes_properties.
   Qed.
 End semtypes_properties.
 
-Section environment_properties.
-  Context `{relocG Σ}.
-  Implicit Types A B : lty2 Σ.
-  Implicit Types Γ : gmap string (lty2 Σ).
-
-  Lemma env_ltyped2_lookup Γ vs x A :
-    Γ !! x = Some A →
-    ⟦ Γ ⟧* vs -∗ ∃ v1 v2, ⌜ vs !! x = Some (v1,v2) ⌝ ∧ A v1 v2.
-  Proof.
-    iIntros (HΓx) "[Hlookup HΓ]". iDestruct "Hlookup" as %Hlookup.
-    destruct (proj1 (Hlookup x)) as [v Hx]; eauto.
-    iExists v.1,v.2. iSplit; first by destruct v.
-    iApply (big_sepM_lookup _ _ x (A,v) with "HΓ").
-    by rewrite map_lookup_zip_with HΓx /= Hx.
-  Qed.
-
-  Lemma env_ltyped2_insert Γ vs x A v1 v2 :
-    A v1 v2 -∗ ⟦ Γ ⟧* vs -∗
-    ⟦ (binder_insert x A Γ) ⟧* (binder_insert x (v1,v2) vs).
-  Proof.
-    destruct x as [|x]=> /=; first by auto.
-    iIntros "#HA [Hlookup #HΓ]". iDestruct "Hlookup" as %Hlookup. iSplit.
-    - iPureIntro=> y. rewrite !lookup_insert_is_Some'. naive_solver.
-    - rewrite -map_insert_zip_with. by iApply big_sepM_insert_2.
-  Qed.
-
-  Lemma env_ltyped2_empty :
-    ⟦ ∅ ⟧* ∅.
-  Proof.
-    iSplit.
-    - iPureIntro=> y. rewrite !lookup_empty -!not_eq_None_Some. by naive_solver.
-    - by rewrite map_zip_with_empty.
-  Qed.
-
-  Global Instance env_ltyped2_persistent Γ vs : Persistent (⟦ Γ ⟧* vs).
-  Proof. apply _. Qed.
-
-End environment_properties.
-
-Notation "'{' E ';' Γ '}' ⊨ e1 '<<' e2 : A" :=
-  (refines E Γ e1%E e2%E (A)%lty2)
-  (at level 100, E at next level, Γ at next level, e1, e2 at next level,
+Notation "'REL' e1 '<<' e2 '@' E ':' A" :=
+  (refines E e1%E e2%E (A)%lty2)
+  (at level 100, E at next level, e1, e2 at next level,
    A at level 200,
-   format "'[hv' '{' E ';' Γ '}'  ⊨  '/  ' e1  '/' '<<'  '/  ' e2  :  A ']'").
-Notation "Γ ⊨ e1 '<<' e2 : A" :=
-  (refines ⊤ Γ e1%E e2%E (A)%lty2)%I
+   format "'[hv' 'REL'  e1  '/' '<<'  '/  ' e2  '@'  E  :  A ']'").
+Notation "'REL' e1 '<<' e2 ':' A" :=
+  (refines ⊤ e1%E e2%E (A)%lty2)
   (at level 100, e1, e2 at next level,
    A at level 200,
-   format "'[hv' Γ  ⊨  '/  ' e1  '/' '<<'  '/  ' e2  :  A ']'").
+   format "'[hv' 'REL'  e1  '/' '<<'  '/  ' e2  :  A ']'").
 
 (** Properties of the relational interpretation *)
 Section related_facts.
   Context `{relocG Σ}.
 
   (* We need this to be able to open and closed invariants in front of logrels *)
-  Lemma fupd_logrel E1 E2 Γ e e' A :
-    ((|={E1,E2}=> {E2;Γ} ⊨ e << e' : A)
-     -∗ ({E1;Γ} ⊨ e << e' : A))%I.
+  Lemma fupd_logrel E1 E2 e e' A :
+    ((|={E1,E2}=> REL e << e' @ E2 : A)
+     -∗ (REL e << e' @ E1 : A))%I.
   Proof.
     rewrite refines_eq /refines_def.
-    iIntros "H".
-    iIntros (vvs ρ) "#Hs HΓ"; iIntros (j K) "Hj /=".
-    iMod "H" as "H".
-    iApply ("H" with "Hs HΓ Hj").
+    iIntros "H". iIntros (ρ) "#Hs"; iIntros (j K) "Hj /=".
+    iMod "H" as "H". iApply ("H" with "Hs Hj").
   Qed.
 
-  Global Instance elim_fupd_logrel p E1 E2 Γ e e' P A :
+  Global Instance elim_fupd_logrel p E1 E2 e e' P A :
    (* TODO: DF: look at the booleans here *)
    ElimModal True p false (|={E1,E2}=> P) P
-     ({E1;Γ} ⊨ e << e' : A) ({E2;Γ} ⊨ e << e' : A).
+     (REL e << e' @ E1 : A) (REL e << e' @ E2: A).
   Proof.
     rewrite /ElimModal. intros _.
     iIntros "[HP HI]". iApply fupd_logrel.
@@ -376,79 +244,62 @@ Section related_facts.
     iMod "HP"; iModIntro; by iApply "HI".
   Qed.
 
-  Global Instance elim_bupd_logrel p E Γ e e' P A :
+  Global Instance elim_bupd_logrel p E e e' P A :
    ElimModal True p false (|==> P) P
-     ({E;Γ} ⊨ e << e' : A) ({E;Γ} ⊨ e << e' : A).
+     (REL e << e' @ E : A) (REL e << e' @ E : A).
   Proof.
     rewrite /ElimModal (bupd_fupd E).
     apply: elim_fupd_logrel.
   Qed.
 
   (* This + elim_modal_timless_bupd' is useful for stripping off laters of timeless propositions. *)
-  Global Instance is_except_0_logrel E Γ e e' A :
-    IsExcept0 ({E;Γ} ⊨ e << e' : A).
+  Global Instance is_except_0_logrel E e e' A :
+    IsExcept0 (REL e << e' @ E : A).
   Proof.
-    rewrite /IsExcept0.
-    iIntros "HL".
-    iApply fupd_logrel.
-    by iMod "HL".
+    rewrite /IsExcept0. iIntros "HL".
+    iApply fupd_logrel. by iMod "HL".
   Qed.
-
 End related_facts.
-
-(** TODO this is a terrible hack and I should be ashamed of myself.
-    See iris issue 225. *)
-Notation is_closed_expr' := (λ e, ∀ vs, subst_map vs e = e).
 
 Section monadic.
   Context `{relocG Σ}.
 
-  Lemma refines_ret' E Γ e1 e2 A :
-    is_closed_expr' e1 →
-    is_closed_expr' e2 →
-    interp_expr E e1 e2 A -∗ {E;Γ} ⊨ e1 << e2 : A.
-  Proof.
-    iIntros (Hcl1 Hcl2) "HA".
-    rewrite refines_eq /refines_def.
-    iIntros (vvs ρ) "#Hs #HΓ".
-    by rewrite Hcl1 Hcl2.
-  Qed.
+  (* Lemma refines_ret_expr E e1 e2 A : *)
+  (*   interp_expr E e1 e2 A -∗ REL e1 << e2 @ E : A. *)
+  (* Proof. *)
+  (*   iIntros "HA". rewrite refines_eq /refines_def. *)
+  (*   eauto with iFrame. *)
+  (* Qed. *)
 
-  Lemma refines_bind K K' E Γ A A' e e' :
-    ({E;Γ} ⊨ e << e' : A) -∗
+  Lemma refines_bind K K' E A A' e e' :
+    (REL e << e' @ E : A) -∗
     (∀ v v', A v v' -∗
-             ({⊤;Γ} ⊨ fill K (of_val v) << fill K' (of_val v') : A')) -∗
-    ({E;Γ} ⊨ fill K e << fill K' e' : A').
+      (REL fill K (of_val v) << fill K' (of_val v') : A')) -∗
+    (REL fill K e << fill K' e' @ E : A').
   Proof.
     iIntros "Hm Hf".
     rewrite refines_eq /refines_def.
-    iIntros (vvs ρ) "#Hs #HΓ". iSpecialize ("Hm" with "Hs HΓ").
+    iIntros (ρ) "#Hs". iSpecialize ("Hm" with "Hs").
     iIntros (j K₁) "Hj /=".
-    rewrite !subst_map_fill -fill_app.
-    iMod ("Hm" with "Hj") as "Hm".
+    rewrite -fill_app. iMod ("Hm" with "Hj") as "Hm".
     iModIntro. iApply wp_bind.
     iApply (wp_wand with "Hm").
     iIntros (v). iDestruct 1 as (v') "[Hj HA]".
-    change (of_val v')
-      with (subst_map (snd <$> vvs) (of_val v')).
-    rewrite fill_app -!subst_map_fill.
-    iMod ("Hf" with "HA Hs HΓ Hj") as "Hf/=".
-    by rewrite !subst_map_fill /=.
+    rewrite fill_app.
+    by iMod ("Hf" with "HA Hs Hj") as "Hf/=".
   Qed.
 
-  Lemma refines_ret E Γ e1 e2 v1 v2 (A : lty2 Σ) :
+  Lemma refines_ret E e1 e2 v1 v2 (A : lty2 Σ) :
     IntoVal e1 v1 →
     IntoVal e2 v2 →
-    (|={E,⊤}=> A v1 v2) -∗ {E;Γ} ⊨ e1 << e2 : A.
+    (|={E,⊤}=> A v1 v2) -∗ REL e1 << e2 @ E : A.
   Proof.
     iIntros (<-<-) "HA".
     rewrite refines_eq /refines_def.
-    iIntros (vvs ρ) "#Hs #HΓ". simpl.
+    iIntros (ρ) "#Hs". simpl.
     iIntros (j K) "Hj /=".
     iMod "HA" as "HA". iModIntro.
     iApply wp_value. iExists _. by iFrame.
   Qed.
 
 End monadic.
-
-Typeclasses Opaque env_ltyped2.
