theories/typing/interp.v
@@ -4,15 +4,20 @@ From iris.algebra Require Export list.
 From iris.proofmode Require Import tactics.
 From reloc.typing Require Export types.
 From reloc.logic Require Import model.
-From reloc.prelude Require Import tactics asubst.
+From reloc.prelude Require Import properness asubst.
 From Autosubst Require Import Autosubst.
 
+(** * Interpretation of types *)
 Section semtypes.
   Context `{relocG Σ}.
   (** Type-level lambdas are interpreted as closures *)
   (** DF: lty2_forall is defined here because it depends on TApp *)
   Definition lty2_forall (C : lty2 Σ → lty2 Σ) : lty2 Σ := Lty2 (λ w1 w2,
-    □ ∀ A : lty2 Σ, interp_expr ⊤ (TApp w1) (TApp w2) (C A))%I.
+    □ ∀ A : lty2 Σ, (() → C A)%lty2 w1 w2)%I.
+  Lemma lty2_forall_spec (C : lty2 Σ → lty2 Σ) w1 w2 :
+    lty2_forall C w1 w2 -∗ ∀ A, (() → C A)%lty2 w1 w2.
+  Proof. eauto with iFrame. Qed.
+
   Definition lty2_true : lty2 Σ := Lty2 (λ w1 w2, True)%I.
 
   Program Definition ctx_lookup (x : var) : listC (lty2C Σ) -n> (lty2C Σ)
@@ -49,6 +54,11 @@ Section semtypes.
     apply lty2_rec_ne=> X /=.
     apply I. by f_equiv.
   Defined.
+  Next Obligation.
+    intros I τ τ' n Δ Δ' HΔ' ??.
+    rewrite /lty2_forall /lty2_car /=.
+    solve_proper.
+  Defined.
 
   Lemma unboxed_type_sound τ Δ v v' :
     UnboxedType τ →
@@ -78,37 +88,13 @@ Section semtypes.
       + iDestruct "H1" as "[% [% H1]]"; simplify_eq/=.
         rewrite IHHτ2. by iDestruct "H1" as "%"; subst.
   Qed.
-
-  Definition bin_log_related (E : coPset)
-             (Δ : list (lty2 Σ)) (Γ : stringmap type)
-             (e e' : expr) (τ : type) : iProp Σ :=
-    {E;fmap (λ τ, interp τ Δ) Γ} ⊨ e << e' : (interp τ Δ).
-
 End semtypes.
 
-Notation "'{' E ';' Δ ';' Γ '}' ⊨ e '≤log≤' e' : τ" :=
-  (bin_log_related E Δ Γ e%E e'%E (τ)%F)
-  (at level 100, E at next level, Δ at next level, Γ at next level, e, e' at next level,
-   τ at level 200,
-   format "'[hv' '{' E ';'  Δ ';'  Γ '}'  ⊨  '/  ' e  '/' '≤log≤'  '/  ' e'  :  τ ']'").
-Notation "'{' Δ ';' Γ '}' ⊨ e '≤log≤' e' : τ" :=
-  (bin_log_related ⊤ Δ Γ e%E e'%E (τ)%F)
-  (at level 100, Δ at next level, Γ at next level, e, e' at next level,
-   τ at level 200,
-   format "'[hv' '{' Δ ';'  Γ '}'  ⊨  '/  ' e  '/' '≤log≤'  '/  ' e'  :  τ ']'").
-
-Section props.
-  Context `{relocG Σ}.
-
-  Lemma fupd_logrel E1 E2 Δ Γ e e' τ :
-    ((|={E1,E2}=> {E2;Δ;Γ} ⊨ e ≤log≤ e' : τ)
-     -∗ {E1;Δ;Γ} ⊨ e ≤log≤ e' : τ)%I.
-  Proof. apply fupd_logrel. Qed.
-
-End props.
-
+(* Shift all the indices in the context by one,
+   used when inserting a new type interpretation in Δ. *)
 Notation "⤉ Γ" := (Autosubst_Classes.subst (ren (+1)%nat) <$> Γ) (at level 10, format "⤉ Γ").
 
+(** ** Properties of the type inrpretation w.r.t. the substitutions *)
 Section interp_ren.
   Context `{relocG Σ}.
   Implicit Types Δ : list (lty2 Σ).
@@ -132,7 +118,9 @@ Section interp_ren.
       { lia. }
       rewrite Hwat. simpl. done.
     - intros v1 v2; unfold lty2_car; simpl; unfold interp_expr;
-        simpl; properness; auto. apply (IHτ (_ :: _)).
+        simpl; properness; auto.
+      rewrite /lty2_car /=. properness; auto.
+      apply interp_expr_proper. apply (IHτ (_ :: _)).
     - intros ??; unfold lty2_car; simpl; properness; auto. apply (IHτ (_ :: _)).
   Qed.
 
@@ -160,7 +148,9 @@ Section interp_ren.
       { by rewrite !lookup_app_l. }
       rewrite !lookup_app_r ;[| lia ..]. do 3 f_equiv. lia.
     - intros ??; simpl; unfold lty2_car; simpl; unfold interp_expr.
-      properness; auto. by apply (IHτ (_ :: _)).
+      properness; auto.
+      rewrite /lty2_car /=. properness; auto.
+      apply interp_expr_proper. apply (IHτ (_ :: _)).
     - intros ??; unfold lty2_car; simpl; properness; auto.
         by apply (IHτ (_ :: _)).
   Qed.
@@ -186,12 +176,106 @@ Section interp_ren.
         asimpl. reflexivity. }
       rewrite !lookup_app_r; [|lia ..]. repeat f_equiv. lia.
     - intros ??. unfold lty2_car; simpl; unfold interp_expr.
-      properness; auto. apply (IHτ (_ :: _)).
+      properness; auto.
+      rewrite /lty2_car /=. properness; auto.
+      apply interp_expr_proper. apply (IHτ (_ :: _)).
     - intros ??; unfold lty2_car; simpl; properness; auto. apply (IHτ (_ :: _)).
   Qed.
 
   Lemma interp_subst Δ2 τ τ' :
     interp τ (interp τ' Δ2 :: Δ2) ≡ interp (τ.[τ'/]) Δ2.
   Proof. apply (interp_subst_up []). Qed.
-
 End interp_ren.
+
+(** * Interpretation of the environments *)
+Section env_typed.
+  Context `{relocG Σ}.
+  Implicit Types A B : lty2 Σ.
+  Implicit Types Γ : gmap string (lty2 Σ).
+
+  (** Substitution [vs] is well-typed w.r.t. [Γ] *)
+  Definition env_ltyped2 (Γ : gmap string (lty2 Σ))
+    (vs : gmap string (val*val)) : iProp Σ :=
+    (⌜ ∀ x, is_Some (Γ !! x) ↔ is_Some (vs !! x) ⌝ ∧
+    [∗ map] i ↦ Avv ∈ map_zip Γ vs, lty2_car Avv.1 Avv.2.1 Avv.2.2)%I.
+
+  Notation "⟦ Γ ⟧*" := (env_ltyped2 Γ).
+
+  Global Instance env_ltyped2_ne n :
+    Proper (dist n ==> (=) ==> dist n) env_ltyped2.
+  Proof.
+    intros Γ Γ' HΓ ? vvs ->.
+    rewrite /env_ltyped2.
+    f_equiv.
+    - f_equiv.
+      split;
+        intros Hvvs x; specialize (HΓ x); rewrite -(Hvvs x);
+          by apply (is_Some_ne n).
+    - apply big_opM_ne2; first apply _.
+      + by intros x A B ->.
+      + apply map_zip_with_ne=>//. apply _.
+  Qed.
+
+  Global Instance env_ltyped2_proper :
+    Proper ((≡) ==> (=) ==> (≡)) env_ltyped2.
+  Proof. solve_proper_from_ne. Qed.
+
+  Lemma env_ltyped2_lookup Γ vs x A :
+    Γ !! x = Some A →
+    ⟦ Γ ⟧* vs -∗ ∃ v1 v2, ⌜ vs !! x = Some (v1,v2) ⌝ ∧ A v1 v2.
+  Proof.
+    iIntros (HΓx) "[Hlookup HΓ]". iDestruct "Hlookup" as %Hlookup.
+    destruct (proj1 (Hlookup x)) as [v Hx]; eauto.
+    iExists v.1,v.2. iSplit; first by destruct v.
+    iApply (big_sepM_lookup _ _ x (A,v) with "HΓ").
+    by rewrite map_lookup_zip_with HΓx /= Hx.
+  Qed.
+
+  Lemma env_ltyped2_insert Γ vs x A v1 v2 :
+    A v1 v2 -∗ ⟦ Γ ⟧* vs -∗
+    ⟦ (binder_insert x A Γ) ⟧* (binder_insert x (v1,v2) vs).
+  Proof.
+    destruct x as [|x]=> /=; first by auto.
+    iIntros "#HA [Hlookup #HΓ]". iDestruct "Hlookup" as %Hlookup. iSplit.
+    - iPureIntro=> y. rewrite !lookup_insert_is_Some'. naive_solver.
+    - rewrite -map_insert_zip_with. by iApply big_sepM_insert_2.
+  Qed.
+
+  Lemma env_ltyped2_empty :
+    ⟦ ∅ ⟧* ∅.
+  Proof.
+    iSplit.
+    - iPureIntro=> y. rewrite !lookup_empty -!not_eq_None_Some. by naive_solver.
+    - by rewrite map_zip_with_empty.
+  Qed.
+
+  Global Instance env_ltyped2_persistent Γ vs : Persistent (⟦ Γ ⟧* vs).
+  Proof. apply _. Qed.
+End env_typed.
+
+Notation "⟦ Γ ⟧*" := (env_ltyped2 Γ).
+
+(** * The semantic typing judgement *)
+Section bin_log_related.
+  Context `{relocG Σ}.
+
+  Definition bin_log_related (E : coPset)
+             (Δ : list (lty2 Σ)) (Γ : stringmap type)
+             (e e' : expr) (τ : type) : iProp Σ :=
+    (∀ vs, ⟦ (λ τ, interp τ Δ) <$> Γ ⟧* vs -∗
+           REL (subst_map (fst <$> vs) e)
+            << (subst_map (snd <$> vs) e') @ E : (interp τ Δ))%I.
+
+End bin_log_related.
+
+Notation "'{' E ';' Δ ';' Γ '}' ⊨ e '≤log≤' e' : τ" :=
+  (bin_log_related E Δ Γ e%E e'%E (τ)%F)
+  (at level 100, E at next level, Δ at next level, Γ at next level, e, e' at next level,
+   τ at level 200,
+   format "'[hv' '{' E ';'  Δ ';'  Γ '}'  ⊨  '/  ' e  '/' '≤log≤'  '/  ' e'  :  τ ']'").
+Notation "'{' Δ ';' Γ '}' ⊨ e '≤log≤' e' : τ" :=
+  (bin_log_related ⊤ Δ Γ e%E e'%E (τ)%F)
+  (at level 100, Δ at next level, Γ at next level, e, e' at next level,
+   τ at level 200,
+   format "'[hv' '{' Δ ';'  Γ '}'  ⊨  '/  ' e  '/' '≤log≤'  '/  ' e'  :  τ ']'").
+
