theories/examples/counter.v
@@ -1,0 +1,241 @@
+From reloc Require Export proofmode.
+From reloc.typing Require Export types interp.
+From reloc.logic Require Import compatibility.
+From reloc.examples Require Import lock.
+From reloc.typing Require Import soundness.
+
+Definition CG_increment : val := λ: "x" "l",
+  acquire "l";;
+  let: "n" := !"x" in
+  "x" <- #1 + "n";;
+  release "l";;
+  "n".
+
+Definition counter_read : val := λ: "x",  !"x".
+
+Definition CG_counter : val := λ: <>,
+  let: "l" := newlock #() in
+  let: "x" := ref #0 in
+  ((λ: <>, CG_increment "x" "l"), (λ: <>, counter_read "x")).
+
+Definition FG_increment : val := rec: "inc" "v" :=
+  let: "c" := !"v" in
+  if: CAS "v" "c" (#1 + "c")
+  then "c"
+  else "inc" "v".
+
+Definition wkincr : val := λ: "l",
+  "l" <- !"l" + #1.
+
+Definition FG_counter : val := λ: <>,
+  let: "x" := ref #0 in
+  ((λ: <>, FG_increment "x"), (λ: <>, counter_read "x")).
+
+Section CG_Counter.
+  Context `{relocG Σ}.
+
+  Lemma CG_increment_r K E t A (x l : loc) (n : nat) :
+    nclose specN ⊆ E →
+    (x ↦ₛ # n -∗ l ↦ₛ #false -∗
+    (x ↦ₛ # (n + 1) -∗ l ↦ₛ #false -∗
+      (REL t << fill K (of_val #n) @ E : A)) -∗
+    REL t << fill K (CG_increment #x #l) @ E : A)%I.
+  Proof.
+    iIntros (?) "Hx Hl Hlog".
+    unfold CG_increment. unlock.
+    repeat rel_pure_r.
+    rel_apply_r (refines_acquire_r with "Hl").
+    iIntros "Hl".
+    repeat rel_pure_r.
+    rel_load_r. repeat rel_pure_r.
+    rel_store_r. repeat rel_pure_r.
+    rel_apply_r (refines_release_r with "Hl").
+    iIntros "Hl". repeat rel_pure_r.
+    replace (n + 1)%Z with (1 + n)%Z; last lia.
+    by iApply ("Hlog" with "Hx Hl").
+  Qed.
+
+  Lemma counter_read_r E K x (n : nat) t A
+    (Hspec : nclose specN ⊆ E) :
+    x ↦ₛ #n -∗
+    (x ↦ₛ #n -∗ REL t << fill K (of_val #n) @ E : A) -∗ (* TODO: of_val *)
+    REL t << fill K (counter_read #x) @ E : A.
+  Proof.
+    iIntros "Hx Hlog".
+    unfold counter_read. unlock. simpl.
+    repeat rel_pure_r. rel_load_r.
+    by iApply "Hlog".
+  Qed.
+
+  Lemma FG_increment_r K E t A (x : loc) (n : nat) :
+    nclose specN ⊆ E →
+    (x ↦ₛ # n -∗
+    (x ↦ₛ #(n + 1) -∗
+      REL t << fill K (of_val #n) @ E : A) -∗
+    REL t << fill K (FG_increment #x) @ E : A)%I.
+  Proof.
+    iIntros (?) "Hx Hlog".
+    unlock FG_increment.
+    repeat rel_pure_r.
+    rel_load_r. repeat rel_pure_r.
+    rel_cas_suc_r.
+    rel_if_r.
+    replace (n + 1)%Z with (1 + n)%Z; last lia.
+    by iApply "Hlog".
+  Qed.
+
+  (* A logically atomic specification for
+     a fine-grained increment with a baked in frame. *)
+  Lemma FG_increment_atomic_l R P E K x t A  :
+    P -∗
+    □ (|={⊤,E}=> ∃ n : nat, x ↦ #n ∗ R n ∗
+       ((x ↦ #n ∗ R n ={E,⊤}=∗ True) ∧
+        (x ↦ #(n+1) ∗ R n -∗ P -∗
+            REL fill K (of_val #n) << t @ E : A)))
+    -∗ REL fill K (FG_increment #x) << t : A.
+  Proof.
+    iIntros "HP #H".
+    iLöb as "IH".
+    rewrite {2}/FG_increment. unlock. simpl.
+    repeat rel_pure_l.
+    iPoseProof "H" as "H2". (* lolwhat *)
+    rel_load_l_atomic.
+    iMod "H" as (n) "[Hx [HR Hrev]]".  iModIntro.
+    iExists #n. iFrame. iNext. iIntros "Hx".
+    iDestruct "Hrev" as "[Hrev _]".
+    iMod ("Hrev" with "[HR Hx]") as "_"; first iFrame.
+    repeat rel_pure_l. rel_cas_l_atomic.
+    iMod "H2" as (n') "[Hx [HR HQ]]". iModIntro. simpl.
+    destruct (decide (n = n')); subst.
+    - iExists #n'. iFrame.
+      iSplitR; eauto. { iDestruct 1 as %Hfoo. exfalso. done. }
+      iIntros "_ !> Hx". simpl.
+      iDestruct "HQ" as "[_ HQ]".
+      replace (n' + 1)%Z with (1 + n')%Z; last by lia. (* TODO :( *)
+      iSpecialize ("HQ" with "[$Hx $HR]").
+      rel_if_true_l. by iApply "HQ".
+    - iExists #n'. iFrame.
+      iSplitL; eauto; last first.
+      { iDestruct 1 as %Hfoo. exfalso. simplify_eq. }
+      iIntros "_ !> Hx". simpl.
+      rel_if_false_l.
+      iDestruct "HQ" as "[HQ _]".
+      iMod ("HQ" with "[$Hx $HR]").
+      rewrite /FG_increment. unlock. simpl.
+      by iApply "IH".
+  Qed.
+
+  (* A similar atomic specification for the counter_read fn *)
+  Lemma counter_read_atomic_l R P E K x t A :
+    P -∗
+    □ (|={⊤,E}=> ∃ n : nat, x ↦ #n ∗ R n ∗
+       (x ↦ #n ∗ R n ={E,⊤}=∗ True) ∧
+        (x ↦ #n ∗ R n -∗ P -∗
+            REL fill K (of_val #n) << t @ E : A))
+    -∗ REL fill K (counter_read #x) << t : A.
+  Proof.
+    iIntros "HP #H".
+    unfold counter_read. unlock. simpl.
+    repeat rel_pure_l. rel_load_l_atomic.
+    iMod "H" as (n) "[Hx [HR Hfin]]". iModIntro.
+    iExists _; iFrame "Hx". iNext.
+    iIntros "Hx".
+    iDestruct "Hfin" as "[_ Hfin]".
+    iApply ("Hfin" with "[Hx HR] HP"). by iFrame.
+  Qed.
+
+
+  Definition counterN : namespace := nroot .@ "counter".
+
+  Definition counter_inv l cnt cnt' : iProp Σ :=
+    (∃ n : nat, l ↦ₛ #false ∗ cnt ↦ #n ∗ cnt' ↦ₛ #n)%I.
+
+  Lemma FG_CG_increment_refinement l cnt cnt' :
+    inv counterN (counter_inv l cnt cnt') -∗
+    REL FG_increment #cnt << CG_increment #cnt' #l : lty2_int.
+  Proof.
+    iIntros "#Hinv".
+    rel_apply_l
+      (FG_increment_atomic_l
+              (fun n => (l ↦ₛ #false) ∗ cnt' ↦ₛ #n)%I
+              True%I); first done.
+    iAlways. iInv counterN as ">Hcnt" "Hcl". iModIntro.
+    iDestruct "Hcnt" as (n) "(Hl & Hcnt & Hcnt')".
+    iExists _; iFrame.
+    iSplit.
+    - iIntros "(Hcnt & Hl & Hcnt')".
+      iApply ("Hcl" with "[-]").
+      iNext. iExists _. iFrame.
+    - iIntros "(Hcnt & Hl & Hcnt') _".
+      rel_apply_r (CG_increment_r with "Hcnt' Hl").
+      iIntros "Hcnt' Hl".
+      iMod ("Hcl" with "[-]").
+      { iNext. iExists (n+1); iFrame.
+        rewrite !Nat2Z.inj_add. by iFrame. }
+      rel_values.
+  Qed.
+
+  Lemma counter_read_refinement l cnt cnt' :
+    inv counterN (counter_inv l cnt cnt') -∗
+    REL counter_read #cnt << counter_read #cnt' : lty2_int.
+  Proof.
+    iIntros "#Hinv".
+    rel_apply_l
+      (counter_read_atomic_l
+         (fun n => (l ↦ₛ #false) ∗ cnt' ↦ₛ #n)%I
+         True%I); first done.
+    iAlways. iInv counterN as (n) "[>Hl [>Hcnt >Hcnt']]" "Hclose".
+    iModIntro.
+    iExists n. iFrame "Hcnt Hcnt' Hl".
+    iSplit.
+    - iIntros "(Hcnt & Hl & Hcnt')". iApply "Hclose".
+      iNext. iExists n. by iFrame.
+    - iIntros "(Hcnt & Hl & Hcnt') _ /=".
+      rel_apply_r (counter_read_r with "Hcnt'").
+      iIntros "Hcnt'".
+      iMod ("Hclose" with "[Hl Hcnt Hcnt']"); simpl.
+      { iNext. iExists _. by iFrame. }
+      rel_values.
+  Qed.
+
+  Lemma FG_CG_counter_refinement :
+    REL FG_counter << CG_counter : (() → (() → lty2_int) × (() → lty2_int))%lty2.
+  Proof.
+    unfold FG_counter, CG_counter. unlock.
+    iApply refines_arrow_val.
+    iAlways. iIntros (? ?) "_"; simplify_eq/=.
+    unlock. rel_rec_l. rel_rec_r.
+    rel_apply_r refines_newlock_r; auto.
+    iIntros (l) "Hl".
+    repeat rel_pure_r.
+    rel_alloc_r cnt' as "Hcnt'".
+    rel_alloc_l cnt as "Hcnt". simpl.
+
+    (* establishing the invariant *)
+    iAssert (counter_inv l cnt cnt')
+      with "[Hl Hcnt Hcnt']" as "Hinv".
+    { iExists 0. by iFrame. }
+    iMod (inv_alloc counterN with "[Hinv]") as "#Hinv"; trivial.
+
+    (* TODO: here we have to do /exactly/ 4 steps.
+       The next step will reduce `(Val v1, Val v2)` to `Val (v1, v2)`,
+       and the compatibility rule wouldn't be applicable *)
+    do 4 rel_pure_r. do 4 rel_pure_l.
+    iApply refines_pair .
+    - iApply refines_arrow_val.
+      iAlways. iIntros (? ?) "_". rel_seq_l; rel_seq_r.
+      iApply (FG_CG_increment_refinement with "Hinv").
+    - iApply refines_arrow_val.
+      iAlways. iIntros (? ?) "_". rel_seq_l; rel_seq_r.
+      iApply (counter_read_refinement with "Hinv").
+  Qed.
+End CG_Counter.
+
+Theorem counter_ctx_refinement :
+  ∅ ⊨ FG_counter ≤ctx≤ CG_counter :
+         TArrow TUnit (TProd (TArrow TUnit TNat) (TArrow TUnit TNat)).
+Proof.
+  eapply (logrel_ctxequiv relocΣ).
+  iIntros (? Δ vs) "#Hvs".
+  iApply FG_CG_counter_refinement.
+Qed.
