theories/logic/compatibility.v
@@ -1,0 +1,61 @@
+(* ReLoC -- Relational logic for fine-grained concurrency *)
+(** Compataibility rules *)
+From iris.proofmode Require Import tactics.
+From iris.algebra Require Import list.
+From iris.program_logic Require Import ectx_lifting.
+From iris.heap_lang Require Import proofmode.
+From reloc.logic Require Export model rules.
+From reloc.logic Require Import proofmode.tactics proofmode.spec_tactics model.
+
+Section compatibility.
+  Context `{relocG Σ}.
+
+  Local Ltac value_case :=
+    try rel_pure_l; try rel_pure_r; rel_values.
+
+  Local Tactic Notation "rel_bind_ap" uconstr(e1) uconstr(e2) constr(IH) ident(v) ident(w) constr(Hv):=
+    rel_bind_l e1;
+    rel_bind_r e2;
+    iApply (refines_bind with IH);
+    iIntros (v w) Hv; simpl.
+
+  Lemma refines_pair e1 e2 e1' e2' A B :
+    (REL e1 << e1' : A) -∗
+    (REL e2 << e2' : B) -∗
+    REL (e1, e2) << (e1', e2') : A × B.
+  Proof.
+    iIntros "IH1 IH2".
+    rel_bind_ap e2 e2' "IH2" v2 v2' "Hvv2".
+    rel_bind_ap e1 e1' "IH1" v1 v1' "Hvv1".
+    value_case.
+    iExists _, _, _, _; eauto.
+  Qed.
+
+  Lemma refines_app e1 e2 e1' e2' A B :
+    (REL e1 << e1' : (A → B)) -∗
+    (REL e2 << e2' : A) -∗
+    REL App e1 e2 << App e1' e2' : B.
+  Proof.
+    iIntros "IH1 IH2".
+    rel_bind_ap e2 e2' "IH2" v v' "Hvv".
+    rel_bind_ap e1 e1' "IH1" f f' "Hff".
+    rewrite interp_val_arrow. by iApply "Hff".
+  Qed.
+
+  Lemma refines_fork e e' E :
+    ↑relocN ⊆ E →
+    (REL e << e' @ E : ()) -∗
+    REL Fork e << Fork e' @ E : ().
+  Proof.
+    iIntros (?) "IH".
+    rewrite refines_eq /refines_def.
+    iIntros (ρ) "#Hρ"; iIntros (j K) "Hj /=".
+    tp_fork j as i "Hi".
+    iSpecialize ("IH" with "Hρ"). unfold interp_expr.
+    iMod ("IH" $! i [] with "Hi") as "IH".
+    iApply (wp_fork with "[-Hj]").
+    - iNext. iApply (wp_wand with "IH"). eauto.
+    - iExists #(); eauto.
+  Qed.
+
+End compatibility.
