theories/logic/rules.v
@@ -19,123 +19,101 @@ Section rules.
 
   (** ** Forward reductions on the LHS *)
 
-  Lemma refines_pure_l Γ n
+  Lemma refines_pure_l n
     (K' : list ectx_item) e e' t A ϕ :
-    PureClosed ϕ n e e' →
+    PureExec ϕ n e e' →
     ϕ →
-    ▷^n (Γ ⊨ fill K' e' << t : A)
-    ⊢ Γ ⊨ fill K' e << t : A.
+    ▷^n (REL fill K' e' << t : A)
+    ⊢ REL fill K' e << t : A.
   Proof.
     intros Hpure Hϕ.
     rewrite refines_eq /refines_def.
-    iIntros "IH" (vvs ρ) "#Hs HΓ"; iIntros (j K) "Hj /=".
-    rewrite subst_map_fill.
-    iApply wp_pure_step_later; [ | apply Hϕ | ].
-    { apply pure_exec_ctx; first apply _.
-      apply pureexec_subst_map. }
-    iModIntro. iNext. iApply fupd_wp.
-    iSpecialize ("IH" with "Hs HΓ Hj").
-    by rewrite subst_map_fill.
+    iIntros "IH" (ρ) "#Hs"; iIntros (j K) "Hj /=".
+    iModIntro. wp_pures.
+    iApply fupd_wp. iApply ("IH" with "Hs Hj").
   Qed.
 
-  Lemma refines_masked_l E Γ n
+  Lemma refines_masked_l E n
     (K' : list ectx_item) e e' t A ϕ :
-    PureClosed ϕ n e e' →
+    PureExec ϕ n e e' →
     ϕ →
-    ({E;Γ} ⊨ fill K' e' << t : A)
-    ⊢ {E;Γ} ⊨ fill K' e << t : A.
+    (REL fill K' e' << t @ E : A)
+    ⊢ REL fill K' e << t @ E : A.
   Proof.
     intros Hpure Hϕ.
     rewrite refines_eq /refines_def.
-    iIntros "IH" (vvs ρ) "#Hs HΓ"; iIntros (j K) "Hj /=".
-    rewrite subst_map_fill.
-    iApply wp_pure_step_later; [ | apply Hϕ | ].
-    { apply pure_exec_ctx; first apply _.
-      apply pureexec_subst_map. }
-    iMod ("IH" with "Hs HΓ Hj") as "IH".
-    iModIntro. iNext.
-    by rewrite subst_map_fill.
+    iIntros "IH" (ρ) "#Hs"; iIntros (j K) "Hj /=".
+    iMod ("IH" with "Hs Hj") as "IH".
+    iModIntro. by wp_pures.
   Qed.
 
-  Lemma refines_wp_l Γ K e1 e2 A :
-    is_closed_expr' e1 →
+  Lemma refines_wp_l K e1 e2 A :
     (WP e1 {{ v,
-        Γ ⊨ fill K (of_val v) << e2 : A }})%I -∗
-    Γ ⊨ fill K e1 << e2 : A.
+        REL fill K (of_val v) << e2 : A }})%I -∗
+    REL fill K e1 << e2 : A.
   Proof.
-    rewrite refines_eq /refines_def =>Hclosed.
+    rewrite refines_eq /refines_def.
     iIntros "He".
-    iIntros (vvs ρ) "#Hs HΓ". iIntros (j K') "Hj /=".
-    rewrite subst_map_fill Hclosed //.
+    iIntros (ρ) "#Hs". iIntros (j K') "Hj /=".
     iModIntro. iApply wp_bind.
     iApply (wp_wand with "He").
     iIntros (v) "Hv".
-    iMod ("Hv" with "Hs [HΓ] Hj"); auto.
-    by rewrite subst_map_fill /=.
+    by iMod ("Hv" with "Hs Hj").
   Qed.
 
-  Lemma refines_atomic_l Γ (E : coPset) K e1 e2 A
+  Lemma refines_atomic_l (E : coPset) K e1 e2 A
         (Hatomic : Atomic WeaklyAtomic e1) :
-    is_closed_expr' e1 →
    (|={⊤,E}=> WP e1 @ E {{ v,
-     {E;Γ} ⊨ fill K (of_val v) << e2 : A }})%I -∗
-   Γ ⊨ fill K e1 << e2 : A.
+     REL fill K (of_val v) << e2 @ E : A }})%I -∗
+   REL fill K e1 << e2 : A.
   Proof.
-    rewrite refines_eq /refines_def => Hclosed.
+    rewrite refines_eq /refines_def.
     iIntros "Hlog".
-    iIntros (vvs ρ) "#Hs HΓ". iIntros (j K') "Hj /=". iModIntro.
-    rewrite subst_map_fill Hclosed //.
-    iApply (wp_bind (fill (subst_map_ctx _ K))).
-    iApply wp_atomic; auto.
+    iIntros (ρ) "#Hs". iIntros (j K') "Hj /=". iModIntro.
+    iApply wp_bind. iApply wp_atomic; auto.
     iMod "Hlog" as "He". iModIntro.
     iApply (wp_wand with "He").
     iIntros (v) "Hlog".
-    iSpecialize ("Hlog" with "Hs [HΓ]"); first by iFrame.
-    iSpecialize ("Hlog" with "Hj"). simpl.
-    rewrite subst_map_fill //.
+    by iApply ("Hlog" with "Hs Hj").
   Qed.
 
   (** ** Forward reductions on the RHS *)
 
-  Lemma refines_pure_r Γ E K' e e' t A n
+  Lemma refines_pure_r E K' e e' t A n
     (Hspec : nclose specN ⊆ E) ϕ :
-    PureClosed ϕ n e e' →
+    PureExec ϕ n e e' →
     ϕ →
-    ({E;Γ} ⊨ t << fill K' e' : A)
-    ⊢ {E;Γ} ⊨ t << fill K' e : A.
+    (REL t << fill K' e' @ E : A)
+    ⊢ REL t << fill K' e @ E : A.
   Proof.
     rewrite refines_eq /refines_def => Hpure Hϕ.
-    iIntros "Hlog". iIntros (vvs ρ) "#Hs HΓ". iIntros (j K) "Hj /=".
-    rewrite subst_map_fill -fill_app.
-    assert (PureExec ϕ n (subst_map (snd <$> vvs) e) (subst_map (snd <$> vvs) e')).
-    { apply pureexec_subst_map. }
+    iIntros "Hlog". iIntros (ρ) "#Hs". iIntros (j K) "Hj /=".
     tp_pure j _; auto.
-    rewrite fill_app -subst_map_fill.
-    iApply ("Hlog" with "Hs HΓ Hj").
+    iApply ("Hlog" with "Hs Hj").
   Qed.
 
-  Lemma refines_step_r Φ Γ E K' e1 e2 A :
-    is_closed_expr' e2 →
+  (* A helper lemma for proving the stateful reductions for the RHS below *)
+  Lemma refines_step_r Φ E K' e1 e2 A :
     (∀ ρ j K, spec_ctx ρ -∗ (j ⤇ fill K e2 ={E}=∗ ∃ v, j ⤇ fill K (of_val v)
                   ∗ Φ v)) -∗
-    (∀ v, Φ v -∗ {E;Γ} ⊨ e1 << fill K' (of_val v) : A) -∗
-    {E;Γ} ⊨ e1 << fill K' e2 : A.
+    (∀ v, Φ v -∗ REL e1 << fill K' (of_val v) @ E : A) -∗
+    REL e1 << fill K' e2 @ E : A.
   Proof.
-    rewrite refines_eq /refines_def=> Hclosed.
+    rewrite refines_eq /refines_def.
     iIntros "He Hlog".
-    iIntros (vvs ρ) "#Hs HΓ". iIntros (j K) "Hj /=".
-    rewrite subst_map_fill -fill_app Hclosed //.
+    iIntros (ρ) "#Hs". iIntros (j K) "Hj /=".
+    rewrite -fill_app.
     iMod ("He" $! ρ j with "Hs Hj") as (v) "[Hj Hv]".
-    iSpecialize ("Hlog" $! v with "Hv Hs HΓ").
-    rewrite fill_app subst_map_fill.
+    iSpecialize ("Hlog" $! v with "Hv Hs").
+    rewrite fill_app.
     by iApply "Hlog".
   Qed.
 
-  Lemma refines_alloc_r Γ E K e v t A
+  Lemma refines_alloc_r E K e v t A
     (Hmasked : nclose specN ⊆ E) :
     IntoVal e v →
-    (∀ l : loc, l ↦ₛ v -∗ {E;Γ} ⊨ t << fill K (of_val #l) : A)%I
-    -∗ {E;Γ} ⊨ t << fill K (ref e) : A.
+    (∀ l : loc, l ↦ₛ v -∗ REL t << fill K (of_val #l) @ E : A)%I
+    -∗ REL t << fill K (ref e) @ E : A.
   Proof.
     intros <-.
     iIntros "Hlog".
@@ -149,11 +127,11 @@ Section rules.
     by iApply "Hlog".
   Qed.
 
-  Lemma refines_load_r Γ E K l q v t A
+  Lemma refines_load_r E K l q v t A
     (Hmasked : nclose specN ⊆ E) :
     l ↦ₛ{q} v -∗
-    (l ↦ₛ{q} v -∗ {E;Γ} ⊨ t << fill K (of_val v) : A)
-    -∗ {E;Γ} ⊨ t << (fill K !#l) : A.
+    (l ↦ₛ{q} v -∗ REL t << fill K (of_val v) @ E : A)
+    -∗ REL t << (fill K !#l) @ E : A.
   Proof.
     iIntros "Hl Hlog".
     pose (Φ := (fun w => ⌜w = v⌝ ∗ l ↦ₛ{q} v)%I).
@@ -166,12 +144,12 @@ Section rules.
     by iApply "Hlog".
   Qed.
 
-  Lemma refines_store_r Γ E K l e e' v v' A
+  Lemma refines_store_r E K l e e' v v' A
     (Hmasked : nclose specN ⊆ E) :
     IntoVal e' v' →
     l ↦ₛ v -∗
-    (l ↦ₛ v' -∗ {E;Γ} ⊨ e << fill K (of_val #()) : A) -∗
-    {E;Γ} ⊨ e << fill K (#l <- e') : A.
+    (l ↦ₛ v' -∗ REL e << fill K (of_val #()) @ E : A) -∗
+    REL e << fill K (#l <- e') @ E : A.
   Proof.
     iIntros (<-) "Hl Hlog".
     pose (Φ := (fun w => ⌜w = #()⌝ ∗ l ↦ₛ v')%I).
@@ -184,15 +162,15 @@ Section rules.
     by iApply "Hlog".
   Qed.
 
-  Lemma refines_cas_fail_r Γ E K l e1 e2 v1 v2 v t A :
+  Lemma refines_cas_fail_r E K l e1 e2 v1 v2 v t A :
     nclose specN ⊆ E →
     IntoVal e1 v1 →
     IntoVal e2 v2 →
     vals_cas_compare_safe v v1 →
     v ≠ v1 →
     l ↦ₛ v -∗
-    (l ↦ₛ v -∗ {E;Γ} ⊨ t << fill K (of_val #false) : A)
-    -∗ {E;Γ} ⊨ t << fill K (CAS #l e1 e2) : A.
+    (l ↦ₛ v -∗ REL t << fill K (of_val #false) @ E : A)
+    -∗ REL t << fill K (CAS #l e1 e2) @ E : A.
   Proof.
     iIntros (?<-<-??) "Hl Hlog".
     pose (Φ := (fun (w : val) => ⌜w = #false⌝ ∗ l ↦ₛ v)%I).
@@ -206,15 +184,15 @@ Section rules.
     by iApply "Hlog".
   Qed.
 
-  Lemma refines_cas_suc_r Γ E K l e1 e2 v1 v2 v t A :
+  Lemma refines_cas_suc_r E K l e1 e2 v1 v2 v t A :
     nclose specN ⊆ E →
     IntoVal e1 v1 →
     IntoVal e2 v2 →
     val_is_unboxed v1 →
     v = v1 →
     l ↦ₛ v -∗
-    (l ↦ₛ v2 -∗ {E;Γ} ⊨ t << fill K (of_val #true) : A)
-    -∗ {E;Γ} ⊨ t << fill K (CAS #l e1 e2) : A.
+    (l ↦ₛ v2 -∗ REL t << fill K (of_val #true) @ E : A)
+    -∗ REL t << fill K (CAS #l e1 e2) @ E : A.
   Proof.
     iIntros (?<-<-??) "Hl Hlog".
     pose (Φ := (fun w => ⌜w = #true⌝ ∗ l ↦ₛ v2)%I).
@@ -228,12 +206,12 @@ Section rules.
     by iApply "Hlog".
   Qed.
 
-  Lemma refines_faa_r Γ E K l e2 (i1 i2 : Z) t A :
+  Lemma refines_faa_r E K l e2 (i1 i2 : Z) t A :
     nclose specN ⊆ E →
     IntoVal e2 #i2 →
     l ↦ₛ #i1 -∗
-    (l ↦ₛ #(i1+i2) -∗ {E;Γ} ⊨ t << fill K (of_val #i1) : A)
-    -∗ {E;Γ} ⊨ t << fill K (FAA #l e2) : A.
+    (l ↦ₛ #(i1+i2) -∗ REL t << fill K (of_val #i1) @ E : A)
+    -∗ REL t << fill K (FAA #l e2) @ E : A.
   Proof.
     iIntros (?<-) "Hl Hlog".
     pose (Φ := (fun w => ⌜w = #i1⌝ ∗ l ↦ₛ #(i1+i2))%I).
@@ -247,17 +225,15 @@ Section rules.
     by iApply "Hlog".
   Qed.
 
-  Lemma refines_fork_r Γ E K (e t : expr) A
-   (Hmasked : nclose specN ⊆ E)
-   (Hclosed : is_closed_expr [] e) :
+  Lemma refines_fork_r E K (e t : expr) A
+   (Hmasked : nclose specN ⊆ E) :
    (∀ i, i ⤇ e -∗
-     {E;Γ} ⊨ t << fill K (of_val #()) : A) -∗
-   {E;Γ} ⊨ t << fill K (Fork e) : A.
+     REL t << fill K (of_val #()) @ E : A) -∗
+   REL t << fill K (Fork e) @ E : A.
   Proof.
     iIntros "Hlog".
     pose (Φ := (fun (v : val) => ∃ i, i ⤇ e ∗ ⌜v = #()⌝%V)%I).
     iApply (refines_step_r Φ with "[]"); cbv[Φ].
-    { intros. by apply subst_map_is_closed_nil. }
     { iIntros (ρ j K') "#Hspec Hj".
       tp_fork j as i "Hi".
       iModIntro. iExists #(). iFrame. eauto.
@@ -267,12 +243,12 @@ Section rules.
   Qed.
 
   (** ** Primitive structural rules *)
-  Lemma refines_spec_ctx Γ E e e' A :
-    ((∃ ρ, spec_ctx ρ) -∗ {E;Γ} ⊨ e << e' : A) -∗
-    ({E;Γ} ⊨ e << e' : A).
+  Lemma refines_spec_ctx E e e' A :
+    ((∃ ρ, spec_ctx ρ) -∗ REL e << e' @ E : A) -∗
+    (REL e << e' @ E : A).
   Proof.
     rewrite refines_eq /refines_def.
-    iIntros "Hctx". iIntros (vvs ρ') "#Hspec".
+    iIntros "Hctx". iIntros (ρ') "#Hspec".
     rewrite -(bi.intuitionistic_intuitionistically (spec_ctx _)).
     rewrite (bi.intuitionistically_sep_dup (spec_ctx _)).
     iDestruct "Hspec" as "[#Hspec #Hspec']".
@@ -281,64 +257,19 @@ Section rules.
     iAssert (∃ ρ, spec_ctx ρ)%I as "Hρ".
     { eauto. }
     iClear "Hspec".
-    iRevert (vvs ρ').
+    iRevert (ρ').
     by iApply "Hctx".
   Qed.
 
-  Lemma refines_var Γ x A :
-    Γ !! x = Some A →
-    Γ ⊨ Var x << Var x : A.
-  Proof.
-    rewrite refines_eq /refines_def.
-    iIntros (? vvs ρ) "#Hs #HΓ"; iIntros (j K) "Hj".
-    iDestruct (env_ltyped2_lookup with "HΓ") as (v1 v2) "[H Hvv]"; first eassumption.
-    iDestruct "H" as %Hvvs.
-    simpl. rewrite !lookup_fmap !Hvvs /=.
-    iModIntro. iApply wp_value. iExists _; by iFrame.
-  Qed.
-
-  Lemma refines_rec Γ (f x : binder) e e' A A' :
-    □(binder_insert f (A → A')%lty2 (binder_insert x A Γ) ⊨ e << e' : A') -∗
-    Γ ⊨ (rec: f x := e) << (rec: f x := e') : (A → A')%lty2.
-  Proof.
-    iIntros "#H".
-    rewrite refines_eq /refines_def.
-    iIntros (vvs ρ) "#Hρ #HΓ /=".
-    iIntros (j K) "Hj". iModIntro.
-    tp_pure j _. wp_pure _.
-    iExists _. iFrame. iLöb as "IH".
-    iAlways. iIntros (v1 v2) "#HA". clear j K.
-    iIntros (j K) "Hj". iModIntro. wp_pures. tp_rec j.
-
-    set (r := (RecV f x (subst_map (binder_delete x (binder_delete f (fst <$> vvs))) e), RecV f x (subst_map (binder_delete x (binder_delete f (snd <$> vvs))) e'))).
-    set (vvs' := binder_insert f r (binder_insert x (v1,v2) vvs)).
-    iSpecialize ("H" $! vvs' with "Hρ [#]").
-    { iApply (env_ltyped2_insert with "IH").
-      iApply (env_ltyped2_insert with "HA").
-      by iFrame. }
-
-    iSpecialize ("H" $! j K). iApply fupd_wp.
-    unfold vvs'.
-    destruct x as [|x], f as [|f];
-      rewrite /= ?fmap_insert ?subst_map_insert //;
-      try by iApply "H".
-    destruct (decide (x = f)) as [->|]; iSimpl in "H".
-    - rewrite !delete_insert_delete !subst_subst !delete_idemp.
-      by iApply "H".
-    - rewrite !delete_insert_ne // subst_map_insert.
-      rewrite !(subst_subst_ne _ x f) // subst_map_insert.
-      by iApply "H".
-  Qed.
-
-  Lemma refines_fork Γ e e' :
-    (Γ ⊨ e << e' : ()%lty2) -∗
-    Γ ⊨ Fork e << Fork e' : ().
+  Lemma refines_fork e e' :
+    (REL e << e' : ()%lty2) -∗
+    REL Fork e << Fork e' : ().
   Proof.
     rewrite refines_eq /refines_def.
     iIntros "H".
-    iIntros (vvs ρ) "#Hs HΓ"; iIntros (j K) "Hj /=".
+    iIntros (ρ) "#Hs"; iIntros (j K) "Hj /=".
     tp_fork j as i "Hi". iModIntro.
-    iSpecialize ("H" with "Hs HΓ").
+    iSpecialize ("H" with "Hs").
     iSpecialize ("H" $! i [] with "Hi"). simpl.
     iApply (wp_fork with "[H]").
     - iNext. iMod "H". iApply (wp_wand with "H"). eauto.
@@ -346,54 +277,63 @@ Section rules.
   Qed.
 
   (** This rule is useful for proving that functions refine each other *)
-  Lemma refines_arrow_val Γ (f x f' x' : binder) e e' eb eb' A A' :
-    e = (RecV f x eb)%E →
-    e' = (RecV f' x' eb')%E →
+  Lemma refines_arrow_val (f x f' x' : binder) eb eb' A A' :
     □(∀ v1 v2, A v1 v2 -∗
-      Γ ⊨ App e (of_val v1) << App e' (of_val v2) : A') -∗
-    Γ ⊨ e << e' : (A → A')%lty2.
+      REL App (RecV f x eb) (of_val v1) << App (RecV f' x' eb') (of_val v2) : A') -∗
+    REL (RecV f x eb) << (RecV f' x' eb') : (A → A')%lty2.
   Proof.
-    iIntros (??) "#H".
-    subst e e'. rewrite refines_eq.
-    (* This is not a consequence of `refines_ret'.
-       For a counterexample, consider a paradoxical [Γ = x :⊥] *)
-    iIntros (vvs ρ) "#Hs #HΓ"; iIntros (j K) "Hj". simpl.
-    iModIntro. iApply wp_value. iExists _; iFrame.
-    iAlways. iIntros (v1 v2) "Hvv".
-    iApply ("H" $! v1 v2 with "Hvv Hs HΓ").
+    iIntros "#H".
+    iApply refines_spec_ctx. iDestruct 1 as (ρ) "#Hs".
+    iApply refines_ret. iModIntro.
+    iModIntro. iIntros (v1 v2) "HA".
+    iSpecialize ("H" with "HA").
+    rewrite refines_eq /refines_def.
+    by iApply "H".
   Qed.
 
-  (* TODO *)
-  (* Lemma interp_val_arrow (A A' : lty2) (v v' : val) ρ : *)
-  (*   spec_ctx ρ -∗ *)
-  (*   (A → A')%lty2 v v' *)
-  (*             ∗-∗ *)
-  (*   (□ (∀ (w w' : val), A w w' *)
-  (*     -∗ ∅ ⊨ v w << v' w' : A'))%I. *)
-  (* Proof. Abort. *)
+  Lemma interp_val_arrow (A A' : lty2 Σ) (v v' : val) :
+    (A → A')%lty2 v v' -∗
+    ((∀ (w w' : val), A w w'
+      -∗ REL v w << v' w' : A'))%I.
+  Proof.
+    iIntros "#H". iIntros (v1 v2) "HA".
+    iSpecialize ("H" with "HA").
+    rewrite refines_eq /refines_def.
+    eauto with iFrame.
+  Qed.
+
+  Lemma interp_arrow_val (A A' : lty2 Σ) (v v' : val) ρ :
+    spec_ctx ρ -∗
+    (□ (∀ (w w' : val), A w w'
+         -∗ REL v w << v' w' : A') -∗
+    (A → A')%lty2 v v')%I.
+  Proof.
+    iIntros "#Hs #H". iModIntro. iIntros (v1 v2) "HA".
+    iSpecialize ("H" with "HA").
+    rewrite refines_eq /refines_def.
+    by iApply "H".
+  Qed.
 
   (** * Some derived (symbolic execution) rules *)
 
   (** ** Stateful reductions on the LHS *)
 
-  Lemma refines_fork_l K Γ E e t A :
-    is_closed_expr [] e →
+  Lemma refines_fork_l K E e t A :
    (|={⊤,E}=> ▷ (WP e {{ _, True }} ∗
-    ({E;Γ} ⊨ fill K (of_val #()) << t : A))) -∗
-   Γ ⊨ fill K (Fork e) << t : A.
+    (REL fill K (of_val #()) << t @ E : A))) -∗
+   REL fill K (Fork e) << t : A.
   Proof.
-    iIntros (?) "Hlog".
+    iIntros "Hlog".
     iApply refines_atomic_l; auto.
-    { intro. by apply subst_map_is_closed_nil. }
     iMod "Hlog" as "[Hsafe Hlog]". iModIntro.
     iApply (wp_fork with "Hsafe"). eauto.
   Qed.
 
-  Lemma refines_alloc_l K Γ E e v t A :
+  Lemma refines_alloc_l K E e v t A :
     IntoVal e v →
     (|={⊤,E}=> ▷ (∀ l : loc, l ↦ v -∗
-           {E;Γ} ⊨ fill K (of_val #l) << t : A))%I
-    -∗ Γ ⊨ fill K (ref e) << t : A.
+           REL fill K (of_val #l) << t @ E : A))%I
+    -∗ REL fill K (ref e) << t : A.
   Proof.
     iIntros (<-) "Hlog".
     iApply refines_atomic_l; auto.
@@ -401,11 +341,11 @@ Section rules.
     iApply (wp_alloc _ _ v); auto.
   Qed.
 
-  Lemma refines_load_l K Γ E l q t A :
+  Lemma refines_load_l K E l q t A :
     (|={⊤,E}=> ∃ v',
       ▷(l ↦{q} v') ∗
-      ▷(l ↦{q} v' -∗ ({E;Γ} ⊨ fill K (of_val v') << t : A)))%I
-    -∗ Γ ⊨ fill K (! #l) << t : A.
+      ▷(l ↦{q} v' -∗ (REL fill K (of_val v') << t @ E : A)))%I
+    -∗ REL fill K (! #l) << t : A.
   Proof.
     iIntros "Hlog".
     iApply refines_atomic_l; auto.
@@ -413,11 +353,11 @@ Section rules.
     iApply (wp_load with "Hl"); auto.
   Qed.
 
-  Lemma refines_store_l K Γ E l e v' t A :
+  Lemma refines_store_l K E l e v' t A :
     IntoVal e v' →
     (|={⊤,E}=> ∃ v, ▷ l ↦ v ∗
-      ▷(l ↦ v' -∗ {E;Γ} ⊨ fill K (of_val #()) << t : A))
-    -∗ Γ ⊨ fill K (#l <- e) << t : A.
+      ▷(l ↦ v' -∗ REL fill K (of_val #()) << t @ E : A))
+    -∗ REL fill K (#l <- e) << t : A.
   Proof.
     iIntros (<-) "Hlog".
     iApply refines_atomic_l; auto.
@@ -425,14 +365,14 @@ Section rules.
     iApply (wp_store _ _ _ _ v' with "Hl"); auto.
   Qed.
 
-  Lemma refines_cas_l K Γ E l e1 e2 v1 v2 t A :
+  Lemma refines_cas_l K E l e1 e2 v1 v2 t A :
     IntoVal e1 v1 →
     IntoVal e2 v2 →
     val_is_unboxed v1 →
     (|={⊤,E}=> ∃ v', ▷ l ↦ v' ∗
-     (⌜v' ≠ v1⌝ -∗ ▷ (l ↦ v' -∗ {E;Γ} ⊨ fill K (of_val #false) << t : A)) ∧
-     (⌜v' = v1⌝ -∗ ▷ (l ↦ v2 -∗ {E;Γ} ⊨ fill K (of_val #true) << t : A)))
-    -∗ Γ ⊨ fill K (CAS #l e1 e2) << t : A.
+     (⌜v' ≠ v1⌝ -∗ ▷ (l ↦ v' -∗ REL fill K (of_val #false) << t @ E : A)) ∧
+     (⌜v' = v1⌝ -∗ ▷ (l ↦ v2 -∗ REL fill K (of_val #true) << t @ E : A)))
+    -∗ REL fill K (CAS #l e1 e2) << t : A.
   Proof.
     iIntros (<-<-?) "Hlog".
     iApply refines_atomic_l; auto.
@@ -450,11 +390,11 @@ Section rules.
       iSpecialize ("Hlog" with "[]"); eauto.
   Qed.
 
-  Lemma refines_faa_l K Γ E l e2 (i2 : Z) t A :
+  Lemma refines_faa_l K E l e2 (i2 : Z) t A :
     IntoVal e2 #i2 →
     (|={⊤,E}=> ∃ (i1 : Z), ▷ l ↦ #i1 ∗
-     ▷ (l ↦ #(i1 + i2) -∗ {E;Γ} ⊨ fill K (of_val #i1) << t : A))
-    -∗ Γ ⊨ fill K (FAA #l e2) << t : A.
+     ▷ (l ↦ #(i1 + i2) -∗ REL fill K (of_val #i1) << t @ E : A))
+    -∗ REL fill K (FAA #l e2) << t : A.
   Proof.
     iIntros (<-) "Hlog".
     iApply refines_atomic_l; auto.
