theories/proofmode.v
@@ -1,3 +1,4 @@
 From iris.heap_lang Require Export lang notation proofmode.
 From iris.proofmode Require Export tactics.
 From reloc.logic Require Export proofmode.tactics proofmode.spec_tactics model.
+From reloc.logic Require Export rules derived compatibility.
