theories/typing/types.v
@@ -1,5 +1,5 @@
 (* ReLoC -- Relational logic for fine-grained concurrency *)
-(** Typing for System F_mu_ref with existential types and concurrency *)
+(** (Syntactic) Typing for System F_mu_ref with existential types and concurrency *)
 From stdpp Require Export stringmap.
 From iris.heap_lang Require Export lang notation metatheory.
 From Autosubst Require Import Autosubst.
